feat: make all targets simple names

src/lake/Lake/Util/Name.lean
@@ -46,6 +46,10 @@ instance [FromJson α] : FromJson (NameMap α) where
 namespace Name
 open Lean.Name
 
+abbrev IsSimple : Name → Prop
+| .str .anonymous _ => True
+| _ => False
+
 @[simp] protected theorem beq_false (m n : Name) : (m == n) = false ↔ ¬ (m = n) := by
   rw [← beq_iff_eq m n]; cases m == n <;> simp (config := { decide := true })
 
@@ -94,3 +98,123 @@ def quoteFrom (ref : Syntax) : Name → Term
 | .anonymous => mkCIdentFrom ref ``anonymous
 | .str p s => mkApp (mkCIdentFrom ref ``mkStr) #[quoteFrom ref p, quote s]
 | .num p v => mkApp (mkCIdentFrom ref ``mkNum) #[quoteFrom ref p, quote v]
+
+end Name
+
+/--
+A subtype of `Lean.Name` that is provably "simple".
+That is, a single-part string name (i.e., `Lean.Name.mkSimple`).
+
+The primary advantage of this type over a plain `String` is that it
+comes with a precomputed `hash` value for quick equality comparisons and
+can be cast into a normal `Name` as a no-op.
+-/
+def SimpleName :=
+  {n : Name // Name.IsSimple n}
+
+namespace SimpleName
+
+abbrev toName (n : SimpleName) : Name :=
+  n.val
+
+instance : Coe SimpleName Name := ⟨toName⟩
+instance : Repr SimpleName := ⟨(·.toName.reprPrec ·)⟩
+
+theorem toName_eq_of_eq {m n : SimpleName} :
+  m = n → m.toName = n.toName
+:= by simp_all
+
+theorem toName_eq_iff_eq {m n : SimpleName} :
+  m.toName = n.toName ↔ m = n
+:= .intro Subtype.eq toName_eq_of_eq
+
+abbrev ofName (n : Name) (h : Name.IsSimple n) : SimpleName :=
+  ⟨n, h⟩
+
+abbrev mk (s : String) : SimpleName :=
+  ofName (.str .anonymous s) True.intro
+
+instance : Inhabited SimpleName := ⟨mk default⟩
+
+instance : Coe String SimpleName := ⟨mk⟩
+instance : CoeDep Name (.str .anonymous s) SimpleName := ⟨mk s⟩
+
+@[inline] protected def hash (n : SimpleName) : UInt64 :=
+  n.toName.hash
+
+instance : Hashable SimpleName := ⟨SimpleName.hash⟩
+
+@[inline] def toString (n : SimpleName) : String :=
+  match n with | ⟨.str _ s, _⟩ => s
+
+instance : ToString SimpleName := ⟨toString⟩
+instance : Coe SimpleName String := ⟨toString⟩
+
+@[simp] theorem string_mk : toString (mk s) = s := rfl
+
+theorem eq_of_toString_eq {n m : SimpleName} :
+  m.toString = n.toString → m = n
+:=
+  match m, n with
+  | ⟨.str .anonymous s, _⟩, ⟨.str .anonymous s', _⟩ =>
+    by intros; simp_all
+
+instance : ToJson SimpleName := ⟨(·.toString)⟩
+instance : FromJson SimpleName := ⟨fun j => mk <$> j.getStr?⟩
+
+protected abbrev beq (m n : SimpleName) : Bool :=
+  m.toName == n.toName
+
+instance : BEq SimpleName := ⟨SimpleName.beq⟩
+
+protected theorem beq_iff_eq {m n : SimpleName} : m == n ↔ m = n := by
+  simp only [BEq.beq]
+  simp [SimpleName.beq, Name.beq_iff_eq, toName_eq_iff_eq]
+
+instance : LawfulBEq SimpleName where
+  eq_of_beq := SimpleName.beq_iff_eq.1
+  rfl := SimpleName.beq_iff_eq.2 rfl
+
+instance : DecidableEq SimpleName :=
+  fun a b => if h : a == b then .isTrue (by simp_all) else .isFalse (by simp_all)
+
+def quickCmp (n₁ n₂ : SimpleName) : Ordering :=
+  match compare n₁.hash n₂.hash with
+  | Ordering.eq => compare n₁.toString n₂.toString
+  | ord => ord
+
+theorem eq_of_quickCmp {n n' : SimpleName} : n.quickCmp n' = .eq → n = n' := by
+  unfold SimpleName.quickCmp
+  intro h_cmp; split at h_cmp
+  next => exact eq_of_toString_eq <| eq_of_cmp h_cmp
+  next => contradiction
+
+theorem quickCmp_rfl {n : SimpleName} : n.quickCmp n = .eq := by
+  unfold SimpleName.quickCmp
+  split <;> exact cmp_rfl
+
+instance : LawfulCmpEq SimpleName SimpleName.quickCmp where
+  eq_of_cmp := eq_of_quickCmp
+  cmp_rfl := quickCmp_rfl
+
+end SimpleName
+
+abbrev SimpleNameSet := RBTree SimpleName SimpleName.quickCmp
+@[inline] def SimpleNameSet.empty : SimpleNameSet := RBTree.empty
+
+abbrev SimpleNameMap (α : Type) := RBMap SimpleName α SimpleName.quickCmp
+@[inline] def SimpleNameMap.empty : SimpleNameMap α := RBMap.empty
+@[inline] def mkSimpleNameMap (α : Type) : SimpleNameMap α := RBMap.empty
+
+instance [ToJson α] : ToJson (SimpleNameMap α) where
+  toJson m := Json.obj <| m.fold (fun n k v => n.insert compare k.toString (toJson v)) .leaf
+
+instance [FromJson α] : FromJson (SimpleNameMap α) where
+  fromJson? j := do (← j.getObj?).foldM (init := {}) fun m k v =>
+    return m.insert (SimpleName.mk k) (← fromJson? v)
+
+abbrev DSimpleNameMap α := DRBMap SimpleName α SimpleName.quickCmp
+@[inline] def SimpleNameMapempty : DNameMap α := DRBMap.empty
+
+abbrev OrdSimpleNameMap α := RBArray SimpleName α SimpleName.quickCmp
+@[inline] def OrdSimpleNameMap.empty : OrdNameMap α := RBArray.empty
