src/lake/Lake/Config/TargetConfig.lean
@@ -9,7 +9,7 @@ import Lake.Build.Store
 namespace Lake
 
 /-- A custom target's declarative configuration. -/
-structure TargetConfig (pkgName name : Name) : Type where
+structure TargetConfig (pkgName name : SimpleName) : Type where
   /-- The target's build function. -/
   build : (pkg : NPackage pkgName) → IndexBuildM (CustomData (pkgName, name))
   /-- The target's resulting build job. -/
@@ -17,7 +17,7 @@ structure TargetConfig (pkgName name : Name) : Type where
   deriving Inhabited
 
 /-- A smart constructor for target configurations that generate CLI targets. -/
-@[inline] def mkTargetJobConfig
+@[inline] def mkTargetJobConfig {name : SimpleName}
 (build : (pkg : NPackage pkgName) → IndexBuildM (BuildJob α))
 [h : FamilyOut CustomData (pkgName, name) (BuildJob α)] : TargetConfig pkgName name where
   build := cast (by rw [← h.family_key_eq_type]) build
@@ -25,12 +25,12 @@ structure TargetConfig (pkgName name : Name) : Type where
 
 /-- A dependently typed configuration based on its registered package and name. -/
 structure TargetDecl where
-  pkg : Name
-  name : Name
+  pkg : SimpleName
+  name : SimpleName
   config : TargetConfig pkg name
 
 hydrate_opaque_type OpaqueTargetConfig TargetConfig pkgName name
 
 /-- Try to find a target configuration in the package with the given name . -/
-def Package.findTargetConfig? (name : Name) (self : Package) : Option (TargetConfig self.name name) :=
+def Package.findTargetConfig? (name : SimpleName) (self : Package) : Option (TargetConfig self.name name) :=
   self.opaqueTargetConfigs.find? name |>.map (·.get)
