src/lake/tests/init/test.sh
@@ -81,10 +81,10 @@ $LAKE -d 123-hello exe 123-hello
 # Test creating packages with components that contain `.`s
 # https://github.com/leanprover/lean4/issues/2999
 
-# this fails on windows for unrelated reasons
+# the unicode name is improperly encoded on windows for unrelated reasons
 if [ "$OSTYPE" != "msys" ]; then
   $LAKE new «A.B».«C.D»
-  $LAKE -d «A-B»-«C-D» exe «a.b-c.d»
+  $LAKE -d A.B-C.D exe a.b-c.d
 fi
 
 # Test creating packages with keyword names
